common/Values.v
@@ -28,14 +28,14 @@ Parameter block : Type.
 Parameter eq_block : forall (x y:block),{x=y}+{x<>y}.
 
 End BLOCK.
-(*
+
 Declare Module Block : BLOCK.
-*)
+(*
 Module Block <: BLOCK.
 Definition block := positive.
 Definition eq_block := peq.
 End Block.
-
+*)
 Definition block := Block.block.
 Definition eq_block := Block.eq_block.
 
